Isabelle chat example (wip)

example_chat.thy
@@ -9,10 +9,12 @@ begin
 
 datatype val =
       String string
+    | UserId int
     | ChatId int
     | MessageId int
     | Bool bool
     | Undef
+    | ListVal "val list"
     
 
 fun stringval where
@@ -26,6 +28,7 @@ record localState =
   ls_content :: val
   ls_to :: val
   ls_id :: val
+  ls_c :: val
 
 definition lsInit :: "localState" where
 "lsInit = \<lparr>
@@ -34,7 +37,8 @@ definition lsInit :: "localState" where
   ls_from = Undef,
   ls_content = Undef,
   ls_to = Undef,
-  ls_id = Undef
+  ls_id = Undef,
+  ls_c = Undef
 \<rparr>"
   
 
@@ -43,64 +47,50 @@ definition sendMessageImpl :: "(localState, val) procedureImpl" where
    (* 0 *) BeginAtomic (ls\<lparr>ls_pc := 1\<rparr>),
    (* 1 *) NewId (\<lambda>x. (ls\<lparr>ls_t := x, ls_pc := 2\<rparr> :: localState)),
    (* 2 *) DbOperation ''message_author_assign'' [ls_t ls, ls_from ls] (\<lambda>r. ls\<lparr>ls_pc := 3\<rparr>),
-   (* 3 *) DbOperation ''message_author_assign'' [ls_t ls, ls_from ls] (\<lambda>r. ls\<lparr>ls_pc := 4\<rparr>),
-   (* 4 *) DbOperation ''message_author_assign'' [ls_t ls, ls_from ls] (\<lambda>r. ls\<lparr>ls_pc := 5\<rparr>),
-   (* 5 *) EndAtomic (ls\<lparr>ls_pc := 6\<rparr>),
-   (* 6 *) Return (ls_t ls)
+   (* 3 *) DbOperation ''message_content_assign'' [ls_t ls, ls_content ls] (\<lambda>r. ls\<lparr>ls_pc := 4\<rparr>),
+   (* 4 *) DbOperation ''message_chat_assign'' [ls_t ls, ls_from ls] (\<lambda>r. ls\<lparr>ls_pc := 5\<rparr>),
+   (* 5 *) DbOperation ''chat_add'' [ls_to ls, ls_t ls] (\<lambda>r. ls\<lparr>ls_pc := 6\<rparr>),
+   (* 6 *) EndAtomic (ls\<lparr>ls_pc := 6\<rparr>),
+   (* 7 *) Return (ls_t ls)
    ] ! ls_pc ls"
 
-definition updateMailImpl :: "(localState, val) procedureImpl" where
-"updateMailImpl ls \<equiv> [
+definition editMessageImpl :: "(localState, val) procedureImpl" where
+"editMessageImpl ls \<equiv> [
    (* 0 *) BeginAtomic (ls\<lparr>ls_pc := 1\<rparr>),
-   (* 1 *) DbOperation ''users_contains_key'' [ls_u ls] (\<lambda>r. ls\<lparr>ls_exists := (r = Bool True), ls_pc := 2 \<rparr>),
-   (* 2 *) LocalStep (if ls_exists ls then ls\<lparr>ls_pc := 3\<rparr> else ls\<lparr>ls_pc := 4\<rparr> ),
-   (* 3 *) DbOperation ''users_mail_assign'' [ls_u ls, String (ls_mail ls)] (\<lambda>r. ls\<lparr>ls_pc := 4\<rparr>),
-   (* 5 *) EndAtomic  (ls\<lparr>ls_pc := 6\<rparr>),
-   (* 6 *) Return Undef
+   (* 1 *) DbOperation ''message_exists'' [ls_id ls] (\<lambda>r. if r = Bool True then ls\<lparr>ls_pc := 2\<rparr> else ls\<lparr>ls_pc := 3\<rparr>),
+   (* 2 *) DbOperation ''message_content_assign'' [ls_id ls, ls_content ls] (\<lambda>r. ls\<lparr>ls_pc := 3\<rparr>),
+   (* 3 *) EndAtomic  (ls\<lparr>ls_pc := 4\<rparr>),
+   (* 4 *) Return Undef
    ] ! ls_pc ls"   
    
-definition removeUserImpl :: "(localState, val) procedureImpl" where
-"removeUserImpl ls \<equiv> [
+definition deleteMessageImpl :: "(localState, val) procedureImpl" where
+"deleteMessageImpl ls \<equiv> [
    (* 0 *) BeginAtomic (ls\<lparr>ls_pc := 1\<rparr>),
-   (* 1 *) DbOperation ''users_remove'' [ls_u ls] (\<lambda>r. ls\<lparr>ls_pc := 2 \<rparr>),
-   (* 2 *) EndAtomic  (ls\<lparr>ls_pc := 3\<rparr>),
-   (* 3 *) Return Undef
-   ] ! ls_pc ls"      
-   
-definition getUserImpl :: "(localState, val) procedureImpl" where
-"getUserImpl ls \<equiv> [
-   (* 0 *) BeginAtomic (ls\<lparr>ls_pc := 1\<rparr>),
-   (* 1 *) DbOperation ''users_contains_key'' [ls_u ls] (\<lambda>r. ls\<lparr>ls_exists := (r = Bool True), ls_pc := 2 \<rparr>),
-   (* 2 *) LocalStep (if ls_exists ls then ls\<lparr>ls_pc := 3\<rparr> else ls\<lparr>ls_pc := 5\<rparr> ),
-   (* 3 *) DbOperation ''users_name_get'' [ls_u ls] (\<lambda>r. ls\<lparr>ls_name := stringval r, ls_pc := 4 \<rparr>),
-   (* 4 *) DbOperation ''users_mail_get'' [ls_u ls] (\<lambda>r. ls\<lparr>ls_mail := stringval r, ls_pc := 5 \<rparr>),
-   (* 5 *) EndAtomic  (ls\<lparr>ls_pc := 6\<rparr>),
-   (* 6 *) Return (if ls_exists ls then Found (ls_name ls) (ls_mail ls) else NotFound )
+   (* 1 *) DbOperation ''message_chat_read'' [ls_id ls] (\<lambda>r. ls\<lparr>ls_pc := 2, ls_c := r\<rparr>),
+   (* 2 *) DbOperation ''chat_remove'' [ls_c ls, ls_id ls] (\<lambda>r. ls\<lparr>ls_pc := 3\<rparr>),
+   (* 3 *) DbOperation ''message_delete'' [ls_id ls] (\<lambda>r. ls\<lparr>ls_pc := 4\<rparr>),
+   (* 4 *) EndAtomic  (ls\<lparr>ls_pc := 5\<rparr>),
+   (* 5 *) Return Undef
    ] ! ls_pc ls"      
    
    
 definition procedures where
 "procedures proc args \<equiv> 
-  if proc = ''registerUser'' then
+  if proc = ''sendMessage'' then
     case args of 
-      [String name, String mail] \<Rightarrow> 
-        Some (lsInit\<lparr>ls_name := name, ls_mail := mail \<rparr> , registerUserImpl)
+      [UserId from, String content, ChatId to] \<Rightarrow> 
+        Some (lsInit\<lparr>ls_from := UserId from, ls_content := String content, ls_to := ChatId to \<rparr> , sendMessageImpl)
       | _ \<Rightarrow> None
-  else if proc = ''updateMail'' then 
+  else if proc = ''editMessage'' then 
     case args of 
-      [UserId u, String mail] \<Rightarrow> 
-        Some (lsInit\<lparr>ls_u := UserId u, ls_mail := mail \<rparr> , updateMailImpl)
+      [MessageId i] \<Rightarrow> 
+        Some (lsInit\<lparr>ls_id := MessageId i \<rparr> , editMessageImpl)
       | _ \<Rightarrow> None
-  else if proc = ''removeUser'' then 
+  else if proc = ''deleteMessage'' then 
     case args of 
-      [UserId u] \<Rightarrow> 
-        Some (lsInit\<lparr>ls_u := UserId u \<rparr> , removeUserImpl)
+      [MessageId i] \<Rightarrow> 
+        Some (lsInit\<lparr>ls_id := MessageId i \<rparr> , deleteMessageImpl)
       | _ \<Rightarrow> None
-  else if proc = ''getUser'' then 
-    case args of 
-      [UserId u] \<Rightarrow> 
-        Some (lsInit\<lparr>ls_u := UserId u \<rparr> , getUserImpl)
-      | _ \<Rightarrow> None  
   else 
     None"
 
@@ -116,52 +106,114 @@ definition latest_mail_assign :: "val operationContext \<Rightarrow> val \<Right
      calls ctxt c1 \<triangleq> Call ''users_mail_assign'' [u, v] Undef
    \<and> (\<forall>c2. calls ctxt c2 \<triangleq> Call ''users_remove'' [u] Undef \<longrightarrow> (c2,c1)\<in>happensBefore ctxt)
    \<and> (\<forall>c2 v'. calls ctxt c2 \<triangleq> Call ''users_mail_assign'' [u] v' \<longrightarrow> \<not>(c1,c2)\<in>happensBefore ctxt)}"   
-   
+
+definition crdtSpec_message_chat_read :: "val list \<Rightarrow> val operationContext \<Rightarrow> val \<Rightarrow> bool" where
+"crdtSpec_message_chat_read args ctxt res \<equiv> \<exists>l.
+  res = ListVal l 
+ \<and> (\<forall>v. v\<in>set l \<longleftrightarrow> 
+   (\<exists>c1. calls ctxt c1 \<triangleq> Call ''message_chat_assign'' (args@[v]) Undef
+     \<and> (\<forall>c2 v'. calls ctxt c2 \<triangleq> Call ''message_chat_assign'' (args@[v']) Undef \<longrightarrow> (c1,c2)\<notin>happensBefore ctxt)
+     \<and> (\<forall>c2. calls ctxt c2 \<triangleq> Call ''message_delete'' args Undef \<longrightarrow> (c2,c1)\<in>happensBefore ctxt)))"
+
+definition crdtSpec_message_author_read :: "val list \<Rightarrow> val operationContext \<Rightarrow> val \<Rightarrow> bool" where
+"crdtSpec_message_author_read args ctxt res \<equiv> \<exists>l.
+  res = ListVal l 
+ \<and> (\<forall>v. v\<in>set l \<longleftrightarrow> 
+   (\<exists>c1. calls ctxt c1 \<triangleq> Call ''message_author_assign'' (args@[v]) Undef
+     \<and> (\<forall>c2 v'. calls ctxt c2 \<triangleq> Call ''message_author_assign'' (args@[v']) Undef \<longrightarrow> (c1,c2)\<notin>happensBefore ctxt)
+     \<and> (\<forall>c2. calls ctxt c2 \<triangleq> Call ''message_delete'' args Undef \<longrightarrow> (c2,c1)\<in>happensBefore ctxt)))"
+
+definition is_message_updateH  where
+ (*:: "val operationContext \<Rightarrow> callId \<Rightarrow> val \<Rightarrow> bool" where *)
+"is_message_updateH state_calls c mid \<equiv> 
+  case state_calls c of 
+     Some (Call upd (mid'#args) _) \<Rightarrow> upd \<in> {''message_author_assign'', ''message_content_assign'', ''message_chat_assign''} \<and> mid = mid' 
+   | _ \<Rightarrow> False"
+
+
+abbreviation is_message_update :: "(val, 'b) operationContext_scheme \<Rightarrow> callId \<Rightarrow> val \<Rightarrow> bool" where
+ (*:: "val operationContext \<Rightarrow> callId \<Rightarrow> val \<Rightarrow> bool" where *)
+"is_message_update ctxt \<equiv> is_message_updateH (calls ctxt)"
+
+definition crdtSpec_message_exists_h :: "val list \<Rightarrow> val operationContext \<Rightarrow> bool" where
+"crdtSpec_message_exists_h args ctxt \<equiv> 
+  \<exists>mId.
+  args = [mId]
+ \<and> (\<exists>c. is_message_update ctxt c mId)
+ \<and> (\<forall>c. calls ctxt c \<triangleq> Call ''message_delete'' args Undef 
+        \<longrightarrow> (\<exists>c'. (c,c')\<in>happensBefore ctxt \<and> is_message_update ctxt c mId))"
+
+definition crdtSpec_message_exists :: "val list \<Rightarrow> val operationContext \<Rightarrow> val \<Rightarrow> bool" where
+"crdtSpec_message_exists args ctxt res \<equiv> 
+  res = Bool (crdtSpec_message_exists_h args ctxt)"
+
+(* ignores map-deletes as they are not used *)
+definition crdtSpec_chat_contains_h :: "val list \<Rightarrow> val operationContext \<Rightarrow> bool" where
+"crdtSpec_chat_contains_h args ctxt \<equiv> 
+  (\<exists>c. calls ctxt c \<triangleq> Call ''chat_add'' args Undef
+      \<and> (\<nexists>c'. calls ctxt c \<triangleq> Call ''chat_remove'' args Undef \<and> (c,c') \<in> happensBefore ctxt))"
+
+definition crdtSpec_chat_contains :: "val list \<Rightarrow> val operationContext \<Rightarrow> val \<Rightarrow> bool" where
+"crdtSpec_chat_contains args ctxt res \<equiv> 
+  res = Bool (crdtSpec_chat_contains_h args ctxt)"
+
+
 definition crdtSpec :: "operation \<Rightarrow> val list \<Rightarrow> val operationContext \<Rightarrow> val \<Rightarrow> bool" where
-"crdtSpec oper args ctxt res \<equiv> 
-  if oper \<in> {''users_name_assign'', ''users_mail_assign'', ''users_remove''} then
-    (* update-operations always return Undef *)
-    res = Undef
-  else if oper = ''users_contains_key'' then
-    res = Bool (\<exists>c1 v. (calls ctxt c1 \<triangleq> Call ''users_name_assign'' (args @ [v]) Undef
-                 \<or> calls ctxt c1 \<triangleq> Call ''users_mail_assign'' (args @ [v]) Undef)
-               \<and> (\<forall>c2. calls ctxt c2 \<triangleq> Call ''users_remove'' args Undef \<longrightarrow> (c2,c1)\<in>happensBefore ctxt))
-  else if oper = ''users_name_get'' then 
-    if latest_name_assign ctxt (hd args) = {} then 
-      res = Undef
-    else
-      res \<in> latest_name_assign ctxt (hd args)
-  else if oper = ''users_mail_get'' then 
-    if latest_mail_assign ctxt (hd args) = {} then 
-      res = Undef
-    else
-      res \<in> latest_mail_assign ctxt (hd args)
-  else
-    False"
-  
+"crdtSpec oper  \<equiv> 
+  if oper = ''message_chat_read'' then crdtSpec_message_chat_read
+  else if oper = ''message_author_read'' then crdtSpec_message_author_read
+  else if oper = ''chat_contains'' then crdtSpec_chat_contains
+  else if oper = ''message_exists'' then crdtSpec_message_exists
+  else 
+    (* other operations are updates and don't have a result *)
+    (\<lambda>args ctxt res. res = Undef)"
+
+
+definition mkContext :: "'a invariantContext \<Rightarrow> 'a operationContext" where
+"mkContext ctxt \<equiv> \<lparr>
+  calls = calls ctxt |` i_visibleCalls ctxt,
+  happensBefore = happensBefore ctxt  |r i_visibleCalls ctxt
+\<rparr>"
+
+lemma mkContext_calls_simps: "calls (mkContext (invContextH state_callOrigin state_transactionOrigin state_transactionStatus state_happensBefore 
+   state_calls state_knownIds state_invocationOp state_invocationRes vis)) 
+= state_calls |` (commitedCallsH state_callOrigin state_transactionStatus \<inter> (vis orElse {}))"
+  by (auto simp add: mkContext_def invContextH_def )
+
+lemma mkContext_calls_eq_simps: "calls (mkContext (invContextH state_callOrigin state_transactionOrigin state_transactionStatus state_happensBefore 
+   state_calls state_knownIds state_invocationOp state_invocationRes vis)) c \<triangleq> x
+\<longleftrightarrow> (isCommittedH state_callOrigin state_transactionStatus c \<and> c \<in> vis orElse {} \<and> state_calls c \<triangleq> x)"
+  by (auto simp add: mkContext_def invContextH_def commitedCallsH_def  restrict_map_def)
+
+lemma mkContext_happensBefore_simps: "happensBefore (mkContext (invContextH state_callOrigin state_transactionOrigin state_transactionStatus state_happensBefore 
+   state_calls state_knownIds state_invocationOp state_invocationRes vis)) 
+= state_happensBefore |r commitedCallsH state_callOrigin state_transactionStatus |r (vis orElse {})"
+  by (auto simp add: mkContext_def invContextH_def )
+
+lemma mkContext_happensBefore_contains_simps: "(c1,c2) \<in> happensBefore (mkContext (invContextH state_callOrigin state_transactionOrigin state_transactionStatus state_happensBefore 
+   state_calls state_knownIds state_invocationOp state_invocationRes vis)) 
+= ( (c1, c2) \<in> state_happensBefore 
+    \<and> isCommittedH state_callOrigin state_transactionStatus c1 \<and> c1 \<in> vis orElse {} 
+    \<and> isCommittedH state_callOrigin state_transactionStatus c2 \<and> c2 \<in> vis orElse {}
+            )"
+  by (auto simp add: mkContext_def invContextH_def commitedCallsH_def restrict_map_def restrict_relation_def)
+
+lemmas mkContext_simps = mkContext_happensBefore_contains_simps mkContext_calls_eq_simps
+
+(* property 1 *)
 definition inv1 :: "val invariantContext \<Rightarrow> bool" where
-"inv1 ctxt \<equiv> \<forall>r g u.
-    i_invocationOp ctxt r \<triangleq> (''removeUser'', [u])
-  \<and> i_invocationOp ctxt g \<triangleq> (''getUser'', [u])
-  \<and> (r,g) \<in> invocation_happensBefore ctxt
-  \<longrightarrow> i_invocationRes ctxt g \<triangleq> NotFound"
-  
+"inv1 ctxt \<equiv> \<forall>c m. crdtSpec_chat_contains_h [c,m] (mkContext ctxt) \<longrightarrow> crdtSpec_message_exists_h [m] (mkContext ctxt)"
+
+(* property 2 *)
 definition inv2 :: "val invariantContext \<Rightarrow> bool" where
-"inv2 ctxt \<equiv> \<forall>u i.
-    i_invocationOp ctxt i \<triangleq> (''removeUser'', [u])
-  \<and> i_invocationRes ctxt i \<noteq> None
-  \<longrightarrow> (\<exists>c. i_callOriginI ctxt c \<triangleq> i \<and> calls ctxt c \<triangleq> Call ''users_remove'' [u] Undef)"
+"inv2 ctxt \<equiv> \<forall>m. crdtSpec_message_exists_h [m] (mkContext ctxt) \<longrightarrow> (\<exists>a. crdtSpec_message_author_read [m] (mkContext ctxt) (ListVal [a]))"
+
+definition inv2_h1 :: "val invariantContext \<Rightarrow> bool" where
+"inv2_h1 ctxt \<equiv> (\<forall>c mId. calls ctxt c \<triangleq> Call ''message_delete'' [mId] Undef \<longrightarrow> (\<nexists>c'. is_message_update ctxt c' mId \<and> (c,c')\<in>happensBefore ctxt ))"
   
-definition inv3 :: "val invariantContext \<Rightarrow> bool" where
-"inv3 ctxt \<equiv> \<not>(\<exists>write delete u v.
-  (calls ctxt write \<triangleq> Call ''users_name_assign'' [u, v] Undef
-    \<or> calls ctxt write \<triangleq> Call ''users_mail_assign'' [u, v] Undef)
-  \<and> (calls ctxt delete \<triangleq> Call ''users_remove'' [u] Undef)
-  \<and> (delete, write) \<in> happensBefore ctxt
-  )"
   
 definition inv :: "val invariantContext \<Rightarrow> bool" where
-"inv ctxt \<equiv> inv1 ctxt \<and> inv2 ctxt \<and> inv3 ctxt"
+"inv ctxt \<equiv> inv1 ctxt \<and> inv2 ctxt \<and> inv2_h1 ctxt"
   
 definition progr :: "(localState, val) prog" where
 "progr \<equiv> \<lparr>
@@ -169,6 +221,64 @@ definition progr :: "(localState, val) prog" where
   procedure = procedures,
   invariant = inv
 \<rparr>"
+
+lemma [simp]: "querySpec progr = crdtSpec" by (simp add: progr_def)
+lemma [simp]: "procedure progr = procedures" by (simp add: progr_def)
+lemma [simp]: "invariant progr = inv" by (simp add: progr_def)
+
+(*
+definition initialStates :: "('localState, 'any) prog \<Rightarrow> invocation \<Rightarrow> ('localState, 'any) state set"  where
+"initialStates progr i \<equiv> {
+    (S\<lparr>localState := (localState S)(i \<mapsto> initState),
+       currentProc := (currentProc S)(i \<mapsto> impl),
+       visibleCalls := (visibleCalls S)(i \<mapsto> {}),
+       invocationOp := (invocationOp S)(i \<mapsto> (procName, args))\<rparr>) 
+ | S procName args initState impl.
+    prog S = progr
+  \<and> procedure progr procName args \<triangleq> (initState, impl)  
+  \<and> uniqueIdsInList args \<subseteq> knownIds S
+  \<and> invariant_all S
+  \<and> state_wellFormed S (*  TODO add wellformed? *)
+  \<and> invocationOp S i = None
+}"
+*)
+
+lemma initialStates_impl:
+  assumes "S \<in> initialStates program i"
+  shows "\<exists>procName args initState impl S_pre.  
+      procedure program procName args \<triangleq> (initState, impl) 
+   \<and> localState S i \<triangleq> initState 
+   \<and> currentProc S i \<triangleq> impl 
+   \<and> invocationOp  S i \<triangleq> (procName, args) 
+   \<and> uniqueIdsInList args \<subseteq> knownIds S
+"
+  using assms by (auto simp add: initialStates_def)
+
+lemma initialStates_prog:
+  assumes "S \<in> initialStates program i"
+  shows "prog S = program"
+  using assms by (auto simp add: initialStates_def)
+
+lemma initialStates_vis:
+  assumes "S \<in> initialStates program i"
+  shows "visibleCalls S i \<triangleq> {}"
+  using assms by (auto simp add: initialStates_def)
+
+lemma initialStates_currentTransaction:
+  assumes "S \<in> initialStates program i"
+  shows "currentTransaction S i = None"
+  using assms apply (auto simp add: initialStates_def)
+  using wellFormed_invoc_notStarted(1) by blast
+
+
+
+
+
+schematic_goal [simp]: "procedure progr = ?p"
+  by (simp add: progr_def)
+
+lemma pc_init[simp]: "ls_pc lsInit = 0"
+  by (simp add: lsInit_def)
 
 
 theorem "programCorrect progr"
@@ -179,18 +289,23 @@ proof (rule show_correctness_via_single_session)
     by (auto simp add: initialStates_def)
   
   show "invariant_all (replissSem1.initialState progr)"
-     by (auto simp add: initialState_def invariant_all_def inv_def inv1_def inv2_def inv3_def invContextH_def)
+    by (auto simp add: initialState_def invariant_all_def inv_def inv1_def inv2_def inv2_h1_def invContextH_def crdtSpec_message_exists_h_def crdtSpec_chat_contains_h_def mkContext_def is_message_updateH_def)
   
      
      
   show "programCorrect_s progr"
   proof (rule show_program_correct_single_invocation)
+
+    text {* First show that the invariant holds for the initial states (beginning of procedures) *}
     show "\<And>S i. S \<in> initialStates progr i \<Longrightarrow> invariant_all S"
     proof (auto simp add: invariant_all_def inv_def)
       fix S i vis
       assume a0: "S \<in> initialStates progr i"
          and vis_cs: "consistentSnapshot S vis"
-      
+
+      have [simp]: "prog S = progr"
+        using a0 by auto
+  
       
       from a0 
       obtain Spre procName args initState impl
@@ -211,51 +326,235 @@ proof (rule show_correctness_via_single_session)
       have pre_inv: "inv (invContextVis Spre vis)"
         by (auto simp add: invariant_all_def `prog Spre = progr` `consistentSnapshot Spre vis`)
         
-      
+
       from pre_inv 
       have "inv1 (invContextVis Spre vis)"
-        using example_userbase.inv_def by blast
+        using inv_def by blast
       thus "inv1 (invContextVis S vis)"
         apply (auto simp add: inv1_def  split: if_splits)
-        apply (auto simp add: invariant_simps)
-        
-        
-        apply (auto simp add: invContextH_def invocation_happensBefore_def i_callOriginI_def )
-        
-        
-        
-        apply (subst(asm) invariantContext.simps)+
-        apply (auto simp add: restrict_relation_def restrict_map_def)
-        
-        find_theorems i_transactionOrigin
-        apply (drule_tac x=r in spec)
-        apply (drule_tac x=g in spec)
-        sorry (* apply (auto simp add: invocation_happensBefore_def) *)
-       
-        (* TODO add simplification rules for "i_invocationOp (invContextVis S vis)" and other fields *)
-        
-      
-      show "inv2 (invContextVis S vis)"
-        using a0 apply (subst(asm) initialStates_def)
-        apply (auto simp add: inv2_def invContextH_def restrict_relation_def restrict_map_def i_callOriginI_def invariantContext.defs split: if_splits option.splits)
-        apply (simp add: state_wellFormed_invocation_before_result)
-        sorry
-        
-      show "inv3 (invContextVis S vis)"
-        using a0 apply (subst(asm) initialStates_def)
-        apply (auto simp add: inv3_def  invContextH_def restrict_relation_def restrict_map_def  split: if_splits)
-        
-        
-      sorry
-    
-    show "\<And>bound S i. S \<in> initialStates progr i \<Longrightarrow> checkCorrect progr S i bound"
-    
-      
-    
-  
-  apply (auto simp add: programCorrect_s_def)
-  apply (auto simp add: prog_def step_s.simps)
+        apply (auto simp add:  crdtSpec_chat_contains_h_def crdtSpec_message_exists_h_def)
+             apply (auto simp add: mkContext_simps  S_def)
+            apply (auto simp add: mkContext_calls_simps )
+        by fastforce+
+
+      from pre_inv 
+      have "inv2 (invContextVis Spre vis)"
+        using inv_def by blast
+      thus "inv2 (invContextVis S vis)"
+        apply (auto simp add: inv2_def  split: if_splits)
+        apply (auto simp add:  crdtSpec_message_exists_h_def crdtSpec_message_author_read_def)
+        by (auto simp add: mkContext_simps  S_def mkContext_calls_simps)
 
 
+         from pre_inv 
+      have "inv2_h1 (invContextVis Spre vis)"
+        using inv_def by blast
+      thus "inv2_h1 (invContextVis S vis)"
+        apply (auto simp add: inv2_h1_def  split: if_splits)
+        by (auto simp add: S_def invContextH_def)
+    qed
+
+
+
+
+    text {* Next, check each procedure: *}
+    show "checkCorrectAll progr S i" if "S \<in> initialStates progr i" for S i
+    proof -
+      from initialStates_impl[OF `S \<in> initialStates progr i`]
+      have "checkCorrectAll progr S i" 
+      proof (auto simp add: procedures_def split: if_splits list.splits val.splits)
+        text {* Procedure editMessage *}
+        fix mId
+        assume a0: "invocationOp S i \<triangleq> (''editMessage'', [MessageId mId])"
+          and a1[simp]: "currentProc S i \<triangleq> editMessageImpl"
+          and a2[simp]: "localState S i \<triangleq> lsInit\<lparr>ls_id := MessageId mId\<rparr>"
+          and a3: "uniqueIdsInList [MessageId mId] \<subseteq> knownIds S"
+
+        have progS[simp]: "prog S = progr"
+          using that by auto 
+        have sameProg[simp]: "prog S' = progr" if "state_monotonicGrowth S S'" for S'
+          using state_monotonicGrowth_prog that by force
+        have [simp]: "currentTransaction S i = None" 
+          using `S \<in> initialStates progr i`  initialStates_currentTransaction by blast 
+        show "checkCorrectAll progr S i"
+        proof (auto simp add: checkCorrectAll_simps editMessageImpl_def; (subst invariant_all_def)?; auto? )
+          text {* We have to show that progress can be made for the query. This is not really necessary for partial correctness but otherwise the program could get stuck.  *}
+          show "\<And>t S'. \<lbrakk>transactionStatus S t = None; invariant_all S'; state_wellFormed S'; state_monotonicGrowth S S'; localState S' i \<triangleq> lsInit\<lparr>ls_id := MessageId mId, ls_pc := Suc 0\<rparr>;
+             currentProc S' i \<triangleq> editMessageImpl; currentTransaction S' i \<triangleq> t; transactionOrigin S' t \<triangleq> i\<rbrakk>
+            \<Longrightarrow> Ex (crdtSpec ''message_exists'' [MessageId mId] (getContext S' i))"
+            by (auto simp add: crdtSpec_def crdtSpec_message_exists_def)
+          show "\<And>t S' c vis.
+             \<lbrakk>transactionStatus S t = None; invariant_all S'; state_wellFormed S'; state_monotonicGrowth S S'; localState S' i \<triangleq> lsInit\<lparr>ls_id := MessageId mId, ls_pc := Suc 0\<rparr>;
+              currentProc S' i \<triangleq> editMessageImpl; currentTransaction S' i \<triangleq> t; transactionOrigin S' t \<triangleq> i; calls S' c = None;
+              crdtSpec ''message_exists'' [MessageId mId] (getContextH (calls S') (happensBefore S') (Some vis)) (Bool True); visibleCalls S' i \<triangleq> vis\<rbrakk>
+             \<Longrightarrow> Ex (crdtSpec ''message_content_assign'' [MessageId mId, ls_content lsInit]
+                      (getContextH (calls S'(c \<mapsto> Call ''message_exists'' [MessageId mId] (Bool True))) (happensBefore S' \<union> vis \<times> {c}) (Some (insert c vis))))"
+            by (auto simp add: crdtSpec_def)
+
+
+
+          show "example_chat.inv (invContextH (callOrigin S'(c \<mapsto> t, ca \<mapsto> t)) (transactionOrigin S') (transactionStatus S'(t \<mapsto> Commited)) (insert (c, ca) (happensBefore S' \<union> vis \<times> {c} \<union> vis \<times> {ca})) (calls S'(c \<mapsto> Call ''message_exists'' [MessageId mId] (Bool True), ca \<mapsto> Call ''message_content_assign'' [MessageId mId, ls_content lsInit] resa)) (knownIds S') (invocationOp S') (invocationRes S') (Some visa))"
+            if c0: "transactionStatus S t = None"
+              and c1: "invariant_all S'"
+              and c2: "state_wellFormed S'"
+              and c3: "state_monotonicGrowth S S'"
+              and c4: "localState S' i \<triangleq> lsInit\<lparr>ls_id := MessageId mId, ls_pc := Suc 0\<rparr>"
+              and c5: "currentProc S' i \<triangleq> editMessageImpl"
+              and c6: "currentTransaction S' i \<triangleq> t"
+              and c7: "transactionOrigin S' t \<triangleq> i"
+              and c8: "calls S' c = None"
+              and c9: "crdtSpec ''message_exists'' [MessageId mId] (getContextH (calls S') (happensBefore S') (Some vis)) (Bool True)"
+              and c10: "visibleCalls S' i \<triangleq> vis"
+              and c11: "ca \<noteq> c"
+              and c12: "calls S' ca = None"
+              and c13: "crdtSpec ''message_content_assign'' [MessageId mId, ls_content lsInit] (getContextH (calls S'(c \<mapsto> Call ''message_exists'' [MessageId mId] (Bool True))) (happensBefore S' \<union> vis \<times> {c}) (Some (insert c vis))) resa"
+              and c14: "consistentSnapshot (S'\<lparr>calls := calls S'(c \<mapsto> Call ''message_exists'' [MessageId mId] (Bool True), ca \<mapsto> Call ''message_content_assign'' [MessageId mId, ls_content lsInit] resa), callOrigin := callOrigin S'(c \<mapsto> t, ca \<mapsto> t), visibleCalls := visibleCalls S'(i \<mapsto> insert ca (insert c vis)), happensBefore := insert (c, ca) (happensBefore S' \<union> vis \<times> {c} \<union> vis \<times> {ca}), localState := localState S'(i \<mapsto> lsInit\<lparr>ls_id := MessageId mId, ls_pc := 4\<rparr>), currentTransaction := (currentTransaction S')(i := None), transactionStatus := transactionStatus S'(t \<mapsto> Commited)\<rparr>) visa"
+            for  t S' c vis ca resa visa
+          proof (auto simp add: inv_def)
+            have [simp]: "prog S' = progr"
+              by (simp add: c3)
+
+            have "consistentSnapshot S' (visa - {c,ca})"
+            proof (auto simp add: consistentSnapshot_def)
+              show "\<And>x. \<lbrakk>x \<in> visa; calls S' x = None; x \<noteq> c\<rbrakk> \<Longrightarrow> x = ca"
+                using c14 by (auto simp add: consistentSnapshot_def)
+
+              from c14 have cc: "causallyConsistent (insert (c, ca) (happensBefore S' \<union> vis \<times> {c} \<union> vis \<times> {ca})) visa"
+                by (auto simp add: consistentSnapshot_def)
+              from c14 have tc: "transactionConsistent (callOrigin S'(c \<mapsto> t, ca \<mapsto> t)) (transactionStatus S'(t \<mapsto> Commited)) visa"
+                by (auto simp add: consistentSnapshot_def)
+
+              show "causallyConsistent (happensBefore S') (visa - {c, ca})"
+              proof (auto simp add: causallyConsistent_def)
+                show "\<And>c1 c2. \<lbrakk>c1 \<in> visa; c1 \<noteq> c; c1 \<noteq> ca; (c2, c1) \<in> happensBefore S'\<rbrakk> \<Longrightarrow> c2 \<in> visa"
+                  by (meson UnCI causallyConsistent_def cc insert_iff)
+                show "\<And>c1. \<lbrakk>c1 \<in> visa; c1 \<noteq> c; c1 \<noteq> ca; (c, c1) \<in> happensBefore S'\<rbrakk> \<Longrightarrow> False"
+                  using c2 c8 wellFormed_happensBefore_calls_l by blast
+                show "\<And>c1. \<lbrakk>c1 \<in> visa; c1 \<noteq> c; c1 \<noteq> ca; (ca, c1) \<in> happensBefore S'\<rbrakk> \<Longrightarrow> False"
+                  using c12 c2 wellFormed_happensBefore_calls_l by blast
+              qed
+
+              show "transactionConsistent (callOrigin S') (transactionStatus S') (visa - {c, ca})"
+              proof (auto simp add: transactionConsistent_def)
+
+                show "transactionStatus S' tx \<triangleq> Commited"
+                  if c0: "cb \<in> visa"
+                    and c1: "cb \<noteq> c"
+                    and c2: "cb \<noteq> ca"
+                    and c3: "callOrigin S' cb \<triangleq> tx"
+                  for  cb tx
+                proof - 
+                  from `callOrigin S' cb \<triangleq> tx` 
+                  have "transactionStatus S tx \<noteq> None"
+                    (* TODO this should be a wf-invariant *)
+                    sorry
+
+                  with `transactionStatus S t = None`
+                  have "tx \<noteq> t"
+                    by blast
+
+                  have "(transactionStatus S'(t \<mapsto> Commited)) tx \<triangleq> Commited"
+                  proof (rule transactionConsistent_Commited[OF tc `cb \<in> visa`])
+                    show "(callOrigin S'(c \<mapsto> t, ca \<mapsto> t)) cb \<triangleq> tx"
+                      by (simp add: c1 c2 c3)
+                    show "(callOrigin S'(c \<mapsto> t, ca \<mapsto> t)) cb \<triangleq> tx"
+                      by (simp add: that)
+                  qed
+                  
+                  with `tx \<noteq> t`
+                  show "transactionStatus S' tx \<triangleq> Commited"
+                    by auto
+                qed
+
+                show "c2 \<in> visa"
+                  if c0: "c1 \<in> visa"
+                    and c1: "c1 \<noteq> c"
+                    and c2: "c1 \<noteq> ca"
+                    and c3: "callOrigin S' c1 = callOrigin S' c2"
+                  for  c1 c2
+                  sorry
+
+                show "False"
+                  if c0: "c1 \<in> visa"
+                    and c1: "c1 \<noteq> c"
+                    and c2: "c1 \<noteq> ca"
+                    and c3: "callOrigin S' c1 = callOrigin S' c"
+                  for  c1
+                  sorry
+
+                show "False"
+                  if c0: "c1 \<in> visa"
+                    and c1: "c1 \<noteq> c"
+                    and c2: "c1 \<noteq> ca"
+                    and c3: "callOrigin S' c1 = callOrigin S' ca"
+                  for  c1
+                  sorry
+              qed
+
+
+
+            from `invariant_all S'` have "inv (invContextVis S' (visa - {c,ca}))"
+              apply (auto simp add: invariant_all_def)
+
+            show "inv1 (invContextH (callOrigin S'(c \<mapsto> t, ca \<mapsto> t)) (transactionOrigin S') (transactionStatus S'(t \<mapsto> Commited)) (insert (c, ca) (happensBefore S' \<union> vis \<times> {c} \<union> vis \<times> {ca}))
+           (calls S'(c \<mapsto> Call ''message_exists'' [MessageId mId] (Bool True), ca \<mapsto> Call ''message_content_assign'' [MessageId mId, ls_content lsInit] resa)) (knownIds S') (invocationOp S')
+           (invocationRes S') (Some visa))"
+              apply (auto simp add: inv1_def crdtSpec_chat_contains_h_def  crdtSpec_message_exists_h_def mkContext_simps)
+              
+              find_theorems calls mkContext
+
+
+
+          show "invariant (prog S') (invContextH (callOrigin S'(c \<mapsto> t, ca \<mapsto> t)) (transactionOrigin S') (transactionStatus S'(t \<mapsto> Commited)) (insert (c, ca) (happensBefore S' \<union> vis \<times> {c} \<union> vis \<times> {ca})) (calls S'(c \<mapsto> Call ''message_exists'' [MessageId mId] (Bool True), ca \<mapsto> Call ''message_content_assign'' [MessageId mId, ls_content lsInit] resa)) (knownIds S') (invocationOp S') (invocationRes S') (Some visa))"
+            if c0: "transactionStatus S t = None"
+              and c1: "invariant_all S'"
+              and c2: "state_wellFormed S'"
+              and c3: "state_monotonicGrowth S S'"
+              and c4: "localState S' i \<triangleq> lsInit\<lparr>ls_id := MessageId mId, ls_pc := Suc 0\<rparr>"
+              and c5: "currentProc S' i \<triangleq> editMessageImpl"
+              and c6: "currentTransaction S' i \<triangleq> t"
+              and c7: "transactionOrigin S' t \<triangleq> i"
+              and c8: "calls S' c = None"
+              and c9: "crdtSpec ''message_exists'' [MessageId mId] (getContextH (calls S') (happensBefore S') (Some vis)) (Bool True)"
+              and c10: "visibleCalls S' i \<triangleq> vis"
+              and c11: "ca \<noteq> c"
+              and c12: "calls S' ca = None"
+              and c13: "crdtSpec ''message_content_assign'' [MessageId mId, ls_content lsInit] (getContextH (calls S'(c \<mapsto> Call ''message_exists'' [MessageId mId] (Bool True))) (happensBefore S' \<union> vis \<times> {c}) (Some (insert c vis))) resa"
+              and c14: "consistentSnapshot (S'\<lparr>calls := calls S'(c \<mapsto> Call ''message_exists'' [MessageId mId] (Bool True), ca \<mapsto> Call ''message_content_assign'' [MessageId mId, ls_content lsInit] resa), callOrigin := callOrigin S'(c \<mapsto> t, ca \<mapsto> t), visibleCalls := visibleCalls S'(i \<mapsto> insert ca (insert c vis)), happensBefore := insert (c, ca) (happensBefore S' \<union> vis \<times> {c} \<union> vis \<times> {ca}), localState := localState S'(i \<mapsto> lsInit\<lparr>ls_id := MessageId mId, ls_pc := 4\<rparr>), currentTransaction := (currentTransaction S')(i := None), transactionStatus := transactionStatus S'(t \<mapsto> Commited)\<rparr>) visa"
+            for  t S' c vis ca resa visa
+          proof (auto simp add: )
+
+
+
+          show "invariant_all
+                  (S'\<lparr>calls := calls S'(c \<mapsto> Call ''message_exists'' [MessageId mId] (Bool True), ca \<mapsto> Call ''message_content_assign'' [MessageId mId, ls_content lsInit] resa),
+                        callOrigin := callOrigin S'(c \<mapsto> t, ca \<mapsto> t), visibleCalls := visibleCalls S'(i \<mapsto> insert ca (insert c vis)),
+                        happensBefore := insert (c, ca) (happensBefore S' \<union> vis \<times> {c} \<union> vis \<times> {ca}), localState := localState S'(i \<mapsto> lsInit\<lparr>ls_id := MessageId mId, ls_pc := 4\<rparr>),
+                        currentTransaction := (currentTransaction S')(i := None), transactionStatus := transactionStatus S'(t \<mapsto> Commited)\<rparr>)"  (is "invariant_all ?newS")
+            if "transactionStatus S t = None" 
+              "invariant_all S'" 
+              "state_wellFormed S'" 
+              "state_monotonicGrowth S S'" 
+              "localState S' i \<triangleq> lsInit\<lparr>ls_id := MessageId mId, ls_pc := Suc 0\<rparr>"
+              "currentProc S' i \<triangleq> editMessageImpl" 
+              "currentTransaction S' i \<triangleq> t" 
+              "transactionOrigin S' t \<triangleq> i" 
+              "calls S' c = None"
+              "crdtSpec ''message_exists'' [MessageId mId] (getContextH (calls S') (happensBefore S') (Some vis)) (Bool True)" "visibleCalls S' i \<triangleq> vis" "ca \<noteq> c" "calls S' ca = None"
+              "crdtSpec ''message_content_assign'' [MessageId mId, ls_content lsInit]
+              (getContextH (calls S'(c \<mapsto> Call ''message_exists'' [MessageId mId] (Bool True))) (happensBefore S' \<union> vis \<times> {c}) (Some (insert c vis))) resa"
+            for t S' c vis ca resa
+          proof (auto simp add: invariant_all_def)
+            fix vis'
+            assume "consistentSnapshot ?newS vis'"
+            show "invariant (prog S')
+             (invContextH (callOrigin S'(c \<mapsto> t, ca \<mapsto> t)) (transactionOrigin S') (transactionStatus S'(t \<mapsto> Commited)) (insert (c, ca) (happensBefore S' \<union> vis \<times> {c} \<union> vis \<times> {ca}))
+               (calls S'(c \<mapsto> Call ''message_exists'' [MessageId mId] (Bool True), ca \<mapsto> Call ''message_content_assign'' [MessageId mId, ls_content lsInit] resa)) (knownIds S')
+               (invocationOp S') (invocationRes S') (Some vis'))"
+              apply (auto simp add: 
+
+
+        
+  qed
 
 end
